vale/specs/interop/Interop.Types.fst
@@ -1,5 +1,5 @@
 module Interop.Types
-module B = LowStar.Buffer
+module MB = LowStar.Monotonic.Buffer
 module W = Words_s
 module L = FStar.List.Tot
 
@@ -20,7 +20,10 @@ let view_n = function
   | TUInt64 -> 8
   | TUInt128 -> 16
 
-let b8 = B.buffer UInt8.t
+[@__reduce__]
+noeq
+type b8 =
+| Buffer: #rrel:MB.srel UInt8.t -> #rel:MB.srel UInt8.t -> b:MB.mbuffer UInt8.t rrel rel -> b8
 
 let disjoint_addr addr1 length1 addr2 length2 =
   (* The first buffer is completely before the second, or the opposite *)
@@ -29,6 +32,6 @@ let disjoint_addr addr1 length1 addr2 length2 =
 
 type addr_map = m:(b8 -> W.nat64){
   (forall (buf1 buf2:b8).{:pattern (m buf1); (m buf2)}
-    B.disjoint buf1 buf2 ==>
-    disjoint_addr (m buf1) (B.length buf1) (m buf2) (B.length buf2)) /\
-  (forall (b:b8).{:pattern (m b)} m b + B.length b < W.pow2_64)}
+    MB.disjoint buf1.b buf2.b ==>
+    disjoint_addr (m buf1) (MB.length buf1.b) (m buf2) (MB.length buf2.b)) /\
+  (forall (b:b8).{:pattern (m b)} m b + MB.length b.b < W.pow2_64)}
